@prefix ob: <https://purl.imsglobal.org/spec/vc/ob/vocab.html#> .
@prefix xsd: <http://www.w3.org/2001/XMLSchema#> .
@prefix dc: <http://purl.org/dc/terms/> .
@prefix owl: <http://www.w3.org/2002/07/owl#> .
@prefix rdfs: <http://www.w3.org/2000/01/rdf-schema#> .
@prefix rdf: <http://www.w3.org/1999/02/22-rdf-syntax-ns#> .

# Ontology definition
ob: a owl:Ontology ;
dc:title """Open Badges 3.0"""@en ;
dc:description """RDFS [[RDF-SCHEMA]] vocabulary used by the Open Badges Data Model 3.0"""@en ;
dc:date "2023-03-29"^^xsd:date ;
.

# Class definitions
ob:Achievement a rdfs:Class ;
rdfs:label "Achievement" ;
rdfs:comment """A collection of information about the accomplishment recognized by the Assertion. Many assertions may be created corresponding to one Achievement."""@en ;
.

ob:AchievementCredential a rdfs:Class ;
rdfs:label "AchievementCredential" ;
rdfs:comment """AchievementCredentials are representations of an awarded achievement, used to share information about a achievement belonging to one earner. Maps to a Verifiable Credential as defined in the [[VC-DATA-MODEL]]. As described in [[[#data-integrity]]], at least one proof mechanism, and the details necessary to evaluate that proof, MUST be expressed for a credential to be a verifiable credential. In the case of an embedded proof, the credential MUST append the proof in the `proof` property."""@en ;
rdfs:subClassOf ob:VerifiableCredential ;
.

ob:AchievementSubject a rdfs:Class ;
rdfs:label "AchievementSubject" ;
rdfs:comment """A collection of information about the recipient of an achievement. Maps to Credential Subject in [[VC-DATA-MODEL]]."""@en ;
rdfs:subClassOf ob:CredentialSubject ;
.

ob:Address a rdfs:Class ;
rdfs:label "Address" ;
rdfs:comment """An address for the described entity."""@en ;
.

ob:Alignment a rdfs:Class ;
rdfs:label "Alignment" ;
rdfs:comment """Describes an alignment between an achievement and a node in an educational framework."""@en ;
.

ob:Criteria a rdfs:Class ;
rdfs:label "Criteria" ;
rdfs:comment """Descriptive metadata about the achievements necessary to be recognized with an assertion of a particular achievement. This data is added to the Achievement class so that it may be rendered when the achievement assertion is displayed, instead of simply a link to human-readable criteria external to the achievement. Embedding criteria allows either enhancement of an external criteria page or increased portability and ease of use by allowing issuers to skip hosting the formerly-required external criteria page altogether. Criteria is used to allow would-be recipients to learn what is required of them to be recognized with an assertion of a particular achievement. It is also used after the assertion is awarded to a recipient to let those inspecting earned achievements know the general requirements that the recipients met in order to earn it."""@en ;
.

ob:EndorsementCredential a rdfs:Class ;
rdfs:label "EndorsementCredential" ;
rdfs:comment """A verifiable credential that asserts a claim about an entity. As described in [[[#data-integrity]]], at least one proof mechanism, and the details necessary to evaluate that proof, MUST be expressed for a credential to be a verifiable credential. In the case of an embedded proof, the credential MUST append the proof in the `proof` property."""@en ;
rdfs:subClassOf ob:VerifiableCredential ;
.

ob:EndorsementSubject a rdfs:Class ;
rdfs:label "EndorsementSubject" ;
rdfs:comment """A collection of information about the subject of the endorsement."""@en ;
rdfs:subClassOf ob:CredentialSubject ;
.

ob:Evidence a rdfs:Class ;
rdfs:label "Evidence" ;
rdfs:comment """Descriptive metadata about evidence related to the achievement assertion. Each instance of the evidence class present in an assertion corresponds to one entity, though a single entry can describe a set of items collectively. There may be multiple evidence entries referenced from an assertion. The narrative property is also in scope of the assertion class to provide an overall description of the achievement related to the assertion in rich text. It is used here to provide a narrative of achievement of the specific entity described. If both the description and narrative properties are present, displayers can assume the narrative value goes into more detail and is not simply a recapitulation of description."""@en ;
.

ob:GeoCoordinates a rdfs:Class ;
rdfs:label "GeoCoordinates" ;
rdfs:comment """The geographic coordinates of a location."""@en ;
.

ob:IdentifierEntry a rdfs:Class ;
rdfs:label "IdentifierEntry" ;
rdfs:comment """IdentifierEntry"""@en ;
.

ob:IdentityObject a rdfs:Class ;
rdfs:label "IdentityObject" ;
rdfs:comment """A collection of information about the recipient of an achievement."""@en ;
.

ob:Image a rdfs:Class ;
rdfs:label "Image" ;
rdfs:comment """Metadata about images that represent assertions, achieve or profiles. These properties can typically be represented as just the id string of the image, but using a fleshed-out document allows for including captions and other applicable metadata."""@en ;
.

ob:Profile a rdfs:Class ;
rdfs:label "Profile" ;
rdfs:comment """A Profile is a collection of information that describes the entity or organization using Open Badges. Issuers must be represented as Profiles, and endorsers, or other entities may also be represented using this vocabulary. Each Profile that represents an Issuer may be referenced in many BadgeClasses that it has defined. Anyone can create and host an Issuer file to start issuing Open Badges. Issuers may also serve as recipients of Open Badges, often identified within an Assertion by specific properties, like their url or contact email address."""@en ;
.

ob:Related a rdfs:Class ;
rdfs:label "Related" ;
rdfs:comment """Identifies a related achievement."""@en ;
.

ob:Result a rdfs:Class ;
rdfs:label "Result" ;
rdfs:comment """Describes a result that was achieved."""@en ;
.

ob:ResultDescription a rdfs:Class ;
rdfs:label "ResultDescription" ;
rdfs:comment """Describes a possible achievement result."""@en ;
.

ob:RubricCriterionLevel a rdfs:Class ;
rdfs:label "RubricCriterionLevel" ;
rdfs:comment """Describes a rubric criterion level."""@en ;
.

ob:Context a rdfs:Class ;
rdfs:label "Context" ;
rdfs:comment """JSON-LD Context. Either a URI with the context definition or a Map with a local context definition MUST be supplied."""@en ;
rdfs:subClassOf ob:URI , ob:Map ;
.

ob:Map a rdfs:Class ;
rdfs:label "Map" ;
rdfs:comment """A map representing an object with unknown, arbitrary properties"""@en ;
.

ob:Multikey a rdfs:Class ;
rdfs:label "Multikey" ;
rdfs:comment """Multikey"""@en ;
.

ob:JWK a rdfs:Class ;
rdfs:label "JWK" ;
rdfs:comment """A JSON Web Key (JWK) formatted according to [[RFC7517]]."""@en ;
.

ob:JWKS a rdfs:Class ;
rdfs:label "JWKS" ;
rdfs:comment """A JWK Set (JWKS) formatted according to [[RFC7517]]."""@en ;
.

ob:AnyIdentifier a rdfs:Class ;
rdfs:label "AnyIdentifier" ;
rdfs:comment """AnyIdentifier"""@en ;
.

ob:IdentifierType a rdfs:Class ;
rdfs:label "IdentifierType" ;
rdfs:comment """IdentifierType"""@en ;
.

ob:GetOpenBadgeCredentialsResponse a rdfs:Class ;
rdfs:label "GetOpenBadgeCredentialsResponse" ;
rdfs:comment """GetOpenBadgeCredentialsResponse"""@en ;
.


# Property definitions
ob:achievedLevel a rdf:Property ;
rdfs:label "achievedLevel" ;
rdfs:comment """If the result represents an achieved rubric criterion level (e.g. Mastered), the value is the `id` of the RubricCriterionLevel in linked ResultDescription."""@en ;
rdfs:domain <ob:Result> ;
rdfs:isDefinedBy <https://purl.imsglobal.org/spec/vc/ob/vocab.html#> ;
.

ob:achievement a rdf:Property ;
rdfs:label "achievement" ;
rdfs:comment """The achievement being awarded."""@en ;
rdfs:range <ob:Achievement> ;
rdfs:domain <ob:AchievementSubject> ;
rdfs:isDefinedBy <https://purl.imsglobal.org/spec/vc/ob/vocab.html#> ;
.

ob:achievementType a rdf:Property ;
rdfs:label "achievementType" ;
rdfs:comment """The type of achievement. This is an extensible vocabulary."""@en ;
rdfs:domain <ob:Achievement> ;
rdfs:isDefinedBy <https://purl.imsglobal.org/spec/vc/ob/vocab.html#> ;
.

ob:activityEndDate a rdf:Property ;
rdfs:label "activityEndDate" ;
rdfs:comment """The datetime the activity ended."""@en ;
rdfs:domain <ob:AchievementSubject> ;
rdfs:isDefinedBy <https://purl.imsglobal.org/spec/vc/ob/vocab.html#> ;
.

ob:activityStartDate a rdf:Property ;
rdfs:label "activityStartDate" ;
rdfs:comment """The datetime the activity started."""@en ;
rdfs:domain <ob:AchievementSubject> ;
rdfs:isDefinedBy <https://purl.imsglobal.org/spec/vc/ob/vocab.html#> ;
.

ob:additionalName a rdf:Property ;
rdfs:label "additionalName" ;
rdfs:comment """Additional name. Includes what is often referred to as 'middle name' in the western world."""@en ;
rdfs:range <https://schema.org/additionalName> ;
rdfs:domain <ob:Profile> ;
rdfs:isDefinedBy <https://purl.imsglobal.org/spec/vc/ob/vocab.html#> ;
.

ob:address a rdf:Property ;
rdfs:label "address" ;
rdfs:comment """An address for the individual or organization."""@en ;
rdfs:range <ob:Address> ;
rdfs:domain <ob:Profile> ;
rdfs:isDefinedBy <https://purl.imsglobal.org/spec/vc/ob/vocab.html#> ;
.

ob:addressCountry a rdf:Property ;
rdfs:label "addressCountry" ;
rdfs:comment """A country."""@en ;
rdfs:range <https://schema.org/addressCountry> ;
rdfs:domain <ob:Address> ;
rdfs:isDefinedBy <https://purl.imsglobal.org/spec/vc/ob/vocab.html#> ;
.

ob:addressCountryCode a rdf:Property ;
rdfs:label "addressCountryCode" ;
rdfs:comment """A country code. The value must be a ISO 3166-1 alpha-2 country code [[ISO3166-1]]."""@en ;
rdfs:domain <ob:Address> ;
rdfs:isDefinedBy <https://purl.imsglobal.org/spec/vc/ob/vocab.html#> ;
.

ob:addressLocality a rdf:Property ;
rdfs:label "addressLocality" ;
rdfs:comment """A locality within the region."""@en ;
rdfs:range <https://schema.org/addressLocality> ;
rdfs:domain <ob:Address> ;
rdfs:isDefinedBy <https://purl.imsglobal.org/spec/vc/ob/vocab.html#> ;
.

ob:addressRegion a rdf:Property ;
rdfs:label "addressRegion" ;
rdfs:comment """A region within the country."""@en ;
rdfs:range <https://schema.org/addressRegion> ;
rdfs:domain <ob:Address> ;
rdfs:isDefinedBy <https://purl.imsglobal.org/spec/vc/ob/vocab.html#> ;
.

ob:alg a rdf:Property ;
rdfs:label "alg" ;
rdfs:comment """The `alg` (algorithm) parameter identifies the algorithm intended for use with the key, such as `RS256` or `PS256`."""@en ;
rdfs:domain <ob:JWK> ;
rdfs:isDefinedBy <https://purl.imsglobal.org/spec/vc/ob/vocab.html#> ;
.

ob:alignment a rdf:Property ;
rdfs:label "alignment" ;
rdfs:comment """In Achievement:An object describing which objectives or educational standards this achievement aligns to, if any."""@en ;
rdfs:comment """In Result:The alignments between this result and nodes in external frameworks. This set of alignments are in addition to the set of alignments defined in the corresponding ResultDescription object."""@en ;
rdfs:comment """In ResultDescription:Alignments between this result description and nodes in external frameworks."""@en ;
rdfs:comment """In RubricCriterionLevel:Alignments between this rubric criterion level and a rubric criterion levels defined in external frameworks."""@en ;
rdfs:range <ob:Alignment> ;
rdfs:domain [ owl:unionOf ( <ob:Achievement> <ob:Result> <ob:ResultDescription> <ob:RubricCriterionLevel> ) ] ;
rdfs:isDefinedBy <https://purl.imsglobal.org/spec/vc/ob/vocab.html#> ;
.

ob:allowedValue a rdf:Property ;
rdfs:label "allowedValue" ;
rdfs:comment """An ordered list of allowed values. The values should be ordered from low to high as determined by the achievement creator."""@en ;
rdfs:domain <ob:ResultDescription> ;
rdfs:isDefinedBy <https://purl.imsglobal.org/spec/vc/ob/vocab.html#> ;
.

ob:audience a rdf:Property ;
rdfs:label "audience" ;
rdfs:comment """A description of the intended audience for a piece of evidence."""@en ;
rdfs:range <https://schema.org/audience> ;
rdfs:domain <ob:Evidence> ;
rdfs:isDefinedBy <https://purl.imsglobal.org/spec/vc/ob/vocab.html#> ;
.

ob:caption a rdf:Property ;
rdfs:label "caption" ;
rdfs:comment """The caption for the image."""@en ;
rdfs:range <https://schema.org/caption> ;
rdfs:domain <ob:Image> ;
rdfs:isDefinedBy <https://purl.imsglobal.org/spec/vc/ob/vocab.html#> ;
.

ob:compactJwsString a rdf:Property ;
rdfs:label "compactJwsString" ;
rdfs:comment """OpenBadgeCredentials that have been signed with the VC-JWT Proof Format MUST be in the `compactJwsString` array."""@en ;
rdfs:domain <ob:GetOpenBadgeCredentialsResponse> ;
rdfs:isDefinedBy <https://purl.imsglobal.org/spec/vc/ob/vocab.html#> ;
.

ob:controller a rdf:Property ;
rdfs:label "controller" ;
rdfs:comment """The identify of the entity that controls this public key."""@en ;
rdfs:domain <ob:Multikey> ;
rdfs:isDefinedBy <https://purl.imsglobal.org/spec/vc/ob/vocab.html#> ;
.

ob:creator a rdf:Property ;
rdfs:label "creator" ;
rdfs:comment """The person or organization that created the achievement definition."""@en ;
rdfs:range <ob:Profile> ;
rdfs:domain <ob:Achievement> ;
rdfs:isDefinedBy <https://purl.imsglobal.org/spec/vc/ob/vocab.html#> ;
.

ob:credential a rdf:Property ;
rdfs:label "credential" ;
rdfs:comment """OpenBadgeCredentials that have not been signed with the VC-JWT Proof Format MUST be in the `credential` array."""@en ;
rdfs:range <ob:AchievementCredential> ;
rdfs:domain <ob:GetOpenBadgeCredentialsResponse> ;
rdfs:isDefinedBy <https://purl.imsglobal.org/spec/vc/ob/vocab.html#> ;
.

ob:credentialSubject a rdf:Property ;
rdfs:label "credentialSubject" ;
rdfs:comment """In AchievementCredential:The recipient of the achievement."""@en ;
rdfs:comment """In EndorsementCredential:The individual, entity, organization, assertion, or achievement that is endorsed and the endorsement comment."""@en ;
rdfs:range [ owl:unionOf ( <ob:AchievementSubject> <ob:EndorsementSubject> ) ] ;
rdfs:domain [ owl:unionOf ( <ob:AchievementCredential> <ob:EndorsementCredential> ) ] ;
rdfs:isDefinedBy <https://purl.imsglobal.org/spec/vc/ob/vocab.html#> ;
.

ob:creditsAvailable a rdf:Property ;
rdfs:label "creditsAvailable" ;
rdfs:comment """Credit hours associated with this entity, or credit hours possible. For example 3.0."""@en ;
rdfs:domain <ob:Achievement> ;
rdfs:isDefinedBy <https://purl.imsglobal.org/spec/vc/ob/vocab.html#> ;
.

ob:creditsEarned a rdf:Property ;
rdfs:label "creditsEarned" ;
rdfs:comment """The number of credits earned, generally in semester or quarter credit hours. This field correlates with the Achievement `creditsAvailable` field."""@en ;
rdfs:domain <ob:AchievementSubject> ;
rdfs:isDefinedBy <https://purl.imsglobal.org/spec/vc/ob/vocab.html#> ;
.

ob:criteria a rdf:Property ;
rdfs:label "criteria" ;
rdfs:comment """Criteria describing how to earn the achievement."""@en ;
rdfs:range <ob:Criteria> ;
rdfs:domain <ob:Achievement> ;
rdfs:isDefinedBy <https://purl.imsglobal.org/spec/vc/ob/vocab.html#> ;
.

ob:cryptosuite a rdf:Property ;
rdfs:label "cryptosuite" ;
rdfs:comment """The `cryptosuite` of the verification method MUST be the string `eddsa-rdf-2022`."""@en ;
rdfs:domain <ob:Multikey> ;
rdfs:isDefinedBy <https://purl.imsglobal.org/spec/vc/ob/vocab.html#> ;
.

ob:dateOfBirth a rdf:Property ;
rdfs:label "dateOfBirth" ;
rdfs:comment """Birthdate of the person."""@en ;
rdfs:domain <ob:Profile> ;
rdfs:isDefinedBy <https://purl.imsglobal.org/spec/vc/ob/vocab.html#> ;
.

ob:description a rdf:Property ;
rdfs:label "description" ;
rdfs:comment """In Achievement:A short description of the achievement."""@en ;
rdfs:comment """In AchievementCredential:The short description of the credential for display purposes in wallets."""@en ;
rdfs:comment """In EndorsementCredential:The short description of the credential for display purposes in wallets."""@en ;
rdfs:comment """In Evidence:A longer description of the evidence."""@en ;
rdfs:comment """In Profile:A short description of the issuer entity or organization."""@en ;
rdfs:comment """In RubricCriterionLevel:Description of the rubric criterion level."""@en ;
rdfs:range <https://schema.org/description> ;
rdfs:domain [ owl:unionOf ( <ob:Achievement> <ob:AchievementCredential> <ob:EndorsementCredential> <ob:Evidence> <ob:Profile> <ob:RubricCriterionLevel> ) ] ;
rdfs:isDefinedBy <https://purl.imsglobal.org/spec/vc/ob/vocab.html#> ;
.

ob:email a rdf:Property ;
rdfs:label "email" ;
rdfs:comment """An email address."""@en ;
rdfs:range <https://schema.org/email> ;
rdfs:domain <ob:Profile> ;
rdfs:isDefinedBy <https://purl.imsglobal.org/spec/vc/ob/vocab.html#> ;
.

ob:endorsement a rdf:Property ;
rdfs:label "endorsement" ;
rdfs:comment """In Achievement:Allows endorsers to make specific claims about the Achievement. These endorsements are signed with a Data Integrity proof format."""@en ;
rdfs:comment """In AchievementCredential:Allows endorsers to make specific claims about the credential, and the achievement and profiles in the credential. These endorsements are signed with a Data Integrity proof format."""@en ;
rdfs:comment """In Profile:Allows endorsers to make specific claims about the individual or organization represented by this profile. These endorsements are signed with a Data Integrity proof format."""@en ;
rdfs:range <ob:EndorsementCredential> ;
rdfs:domain [ owl:unionOf ( <ob:Achievement> <ob:AchievementCredential> <ob:Profile> ) ] ;
rdfs:isDefinedBy <https://purl.imsglobal.org/spec/vc/ob/vocab.html#> ;
.

ob:endorsementComment a rdf:Property ;
rdfs:label "endorsementComment" ;
rdfs:comment """Allows endorsers to make a simple claim in writing about the entity."""@en ;
rdfs:domain <ob:EndorsementSubject> ;
rdfs:isDefinedBy <https://purl.imsglobal.org/spec/vc/ob/vocab.html#> ;
.

ob:endorsementJwt a rdf:Property ;
rdfs:label "endorsementJwt" ;
rdfs:comment """In Achievement:Allows endorsers to make specific claims about the Achievement. These endorsements are signed with the VC-JWT proof format."""@en ;
rdfs:comment """In AchievementCredential:Allows endorsers to make specific claims about the credential, and the achievement and profiles in the credential. These endorsements are signed with the VC-JWT proof format."""@en ;
rdfs:comment """In Profile:Allows endorsers to make specific claims about the individual or organization represented by this profile. These endorsements are signed with the VC-JWT proof format."""@en ;
rdfs:domain [ owl:unionOf ( <ob:Achievement> <ob:AchievementCredential> <ob:Profile> ) ] ;
rdfs:isDefinedBy <https://purl.imsglobal.org/spec/vc/ob/vocab.html#> ;
.

ob:evidence a rdf:Property ;
rdfs:label "evidence" ;
rdfs:comment """A description of the work that the recipient did to earn the achievement. This can be a page that links out to other pages if linking directly to the work is infeasible."""@en ;
rdfs:range <ob:Evidence> ;
rdfs:domain <ob:AchievementCredential> ;
rdfs:isDefinedBy <https://purl.imsglobal.org/spec/vc/ob/vocab.html#> ;
.

ob:familyName a rdf:Property ;
rdfs:label "familyName" ;
rdfs:comment """Family name. In the western world, often referred to as the 'last name' of a person."""@en ;
rdfs:range <https://schema.org/familyName> ;
rdfs:domain <ob:Profile> ;
rdfs:isDefinedBy <https://purl.imsglobal.org/spec/vc/ob/vocab.html#> ;
.

ob:familyNamePrefix a rdf:Property ;
rdfs:label "familyNamePrefix" ;
rdfs:comment """Family name prefix. As used in some locales, this is the leading part of a family name (e.g. 'de' in the name 'de Boer')."""@en ;
rdfs:domain <ob:Profile> ;
rdfs:isDefinedBy <https://purl.imsglobal.org/spec/vc/ob/vocab.html#> ;
.

ob:fieldOfStudy a rdf:Property ;
rdfs:label "fieldOfStudy" ;
rdfs:comment """Category, subject, area of study, discipline, or general branch of knowledge. Examples include Business, Education, Psychology, and Technology."""@en ;
rdfs:domain <ob:Achievement> ;
rdfs:isDefinedBy <https://purl.imsglobal.org/spec/vc/ob/vocab.html#> ;
.

ob:genre a rdf:Property ;
rdfs:label "genre" ;
rdfs:comment """A string that describes the type of evidence. For example, Poetry, Prose, Film."""@en ;
rdfs:range <https://schema.org/genre> ;
rdfs:domain <ob:Evidence> ;
rdfs:isDefinedBy <https://purl.imsglobal.org/spec/vc/ob/vocab.html#> ;
.

ob:geo a rdf:Property ;
rdfs:label "geo" ;
rdfs:comment """The geographic coordinates of the location."""@en ;
rdfs:range <ob:GeoCoordinates> ;
rdfs:domain <ob:Address> ;
rdfs:isDefinedBy <https://purl.imsglobal.org/spec/vc/ob/vocab.html#> ;
.

ob:givenName a rdf:Property ;
rdfs:label "givenName" ;
rdfs:comment """Given name. In the western world, often referred to as the 'first name' of a person."""@en ;
rdfs:range <https://schema.org/givenName> ;
rdfs:domain <ob:Profile> ;
rdfs:isDefinedBy <https://purl.imsglobal.org/spec/vc/ob/vocab.html#> ;
.

ob:hashed a rdf:Property ;
rdfs:label "hashed" ;
rdfs:comment """Whether or not the `identityHash` value is hashed."""@en ;
rdfs:domain <ob:IdentityObject> ;
rdfs:isDefinedBy <https://purl.imsglobal.org/spec/vc/ob/vocab.html#> ;
.

ob:honorificPrefix a rdf:Property ;
rdfs:label "honorificPrefix" ;
rdfs:comment """Honorific prefix(es) preceding a person's name (e.g. 'Dr', 'Mrs' or 'Mr')."""@en ;
rdfs:range <https://schema.org/honorificPrefix> ;
rdfs:domain <ob:Profile> ;
rdfs:isDefinedBy <https://purl.imsglobal.org/spec/vc/ob/vocab.html#> ;
.

ob:honorificSuffix a rdf:Property ;
rdfs:label "honorificSuffix" ;
rdfs:comment """Honorific suffix(es) following a person's name (e.g. 'M.D, PhD')."""@en ;
rdfs:range <https://schema.org/honorificSuffix> ;
rdfs:domain <ob:Profile> ;
rdfs:isDefinedBy <https://purl.imsglobal.org/spec/vc/ob/vocab.html#> ;
.

ob:humanCode a rdf:Property ;
rdfs:label "humanCode" ;
rdfs:comment """The code, generally human readable, associated with an achievement."""@en ;
rdfs:domain <ob:Achievement> ;
rdfs:isDefinedBy <https://purl.imsglobal.org/spec/vc/ob/vocab.html#> ;
.

ob:identifier a rdf:Property ;
rdfs:label "identifier" ;
rdfs:comment """In AchievementSubject:Other identifiers for the recipient of the achievement. Either `id` or at least one `identifier` MUST be supplied."""@en ;
rdfs:comment """In IdentifierEntry:An identifier."""@en ;
rdfs:comment """In AnyIdentifier:An identifier."""@en ;
rdfs:range <ob:IdentityObject> ;
rdfs:domain [ owl:unionOf ( <ob:AchievementSubject> <ob:IdentifierEntry> <ob:AnyIdentifier> ) ] ;
rdfs:isDefinedBy <https://purl.imsglobal.org/spec/vc/ob/vocab.html#> ;
.

ob:identifierType a rdf:Property ;
rdfs:label "identifierType" ;
rdfs:comment """In IdentifierEntry:The identifier type."""@en ;
rdfs:comment """In IdentifierType:The identifier type."""@en ;
rdfs:domain [ owl:unionOf ( <ob:IdentifierEntry> <ob:IdentifierType> ) ] ;
rdfs:isDefinedBy <https://purl.imsglobal.org/spec/vc/ob/vocab.html#> ;
.

ob:identityHash a rdf:Property ;
rdfs:label "identityHash" ;
rdfs:comment """Either the IdentityHash of the identity or the plaintext value. If it's possible that the plaintext transmission and storage of the identity value would leak personally identifiable information where there is an expectation of privacy, it is strongly recommended that an IdentityHash be used."""@en ;
rdfs:domain <ob:IdentityObject> ;
rdfs:isDefinedBy <https://purl.imsglobal.org/spec/vc/ob/vocab.html#> ;
.

ob:identityType a rdf:Property ;
rdfs:label "identityType" ;
rdfs:comment """The identity type."""@en ;
rdfs:domain <ob:IdentityObject> ;
rdfs:isDefinedBy <https://purl.imsglobal.org/spec/vc/ob/vocab.html#> ;
.

ob:image a rdf:Property ;
rdfs:label "image" ;
rdfs:comment """In Achievement:An image representing the achievement."""@en ;
rdfs:comment """In AchievementCredential:The image representing the credential for display purposes in wallets."""@en ;
rdfs:comment """In AchievementSubject:An image representing this user's achievement. If present, this must be a PNG or SVG image, and should be prepared via the 'baking' instructions. An 'unbaked' image for the achievement is defined in the Achievement class and should not be duplicated here."""@en ;
rdfs:comment """In Profile:An image representing the issuer. This must be a PNG or SVG image."""@en ;
rdfs:range <ob:Image> ;
rdfs:domain [ owl:unionOf ( <ob:Achievement> <ob:AchievementCredential> <ob:AchievementSubject> <ob:Profile> ) ] ;
rdfs:isDefinedBy <https://purl.imsglobal.org/spec/vc/ob/vocab.html#> ;
.

ob:key_ops a rdf:Property ;
rdfs:label "key_ops" ;
rdfs:comment """The `key_ops` (key operations) parameter identifies the operation(s) for which the key is intended to be used, such as `sign` (compute digital signature or MAC) or `verify` (verify digital signature or MAC)."""@en ;
rdfs:domain <ob:JWK> ;
rdfs:isDefinedBy <https://purl.imsglobal.org/spec/vc/ob/vocab.html#> ;
.

ob:keys a rdf:Property ;
rdfs:label "keys" ;
rdfs:comment """A JWK Set is a JSON object that represents a set of JWKs."""@en ;
rdfs:range <ob:JWK> ;
rdfs:domain <ob:JWKS> ;
rdfs:isDefinedBy <https://purl.imsglobal.org/spec/vc/ob/vocab.html#> ;
.

ob:kid a rdf:Property ;
rdfs:label "kid" ;
rdfs:comment """The `kid` (key ID) parameter is used to match a specific key."""@en ;
rdfs:domain <ob:JWK> ;
rdfs:isDefinedBy <https://purl.imsglobal.org/spec/vc/ob/vocab.html#> ;
.

ob:kty a rdf:Property ;
rdfs:label "kty" ;
rdfs:comment """The `kty` (key type) parameter identifies the cryptographic algorithm family used with the key, such as `RSA` or `EC`."""@en ;
rdfs:domain <ob:JWK> ;
rdfs:isDefinedBy <https://purl.imsglobal.org/spec/vc/ob/vocab.html#> ;
.

ob:latitude a rdf:Property ;
rdfs:label "latitude" ;
rdfs:comment """The latitude of the location [[WGS84]]."""@en ;
rdfs:range <https://schema.org/latitude> ;
rdfs:domain <ob:GeoCoordinates> ;
rdfs:isDefinedBy <https://purl.imsglobal.org/spec/vc/ob/vocab.html#> ;
.

ob:level a rdf:Property ;
rdfs:label "level" ;
rdfs:comment """The rubric performance level in terms of success."""@en ;
rdfs:domain <ob:RubricCriterionLevel> ;
rdfs:isDefinedBy <https://purl.imsglobal.org/spec/vc/ob/vocab.html#> ;
.

ob:licenseNumber a rdf:Property ;
rdfs:label "licenseNumber" ;
rdfs:comment """The license number that was issued with this credential."""@en ;
rdfs:domain <ob:AchievementSubject> ;
rdfs:isDefinedBy <https://purl.imsglobal.org/spec/vc/ob/vocab.html#> ;
.

ob:longitude a rdf:Property ;
rdfs:label "longitude" ;
rdfs:comment """The longitude of the location [[WGS84]]."""@en ;
rdfs:range <https://schema.org/longitude> ;
rdfs:domain <ob:GeoCoordinates> ;
rdfs:isDefinedBy <https://purl.imsglobal.org/spec/vc/ob/vocab.html#> ;
.

ob:name a rdf:Property ;
rdfs:label "name" ;
rdfs:comment """In Achievement:The name of the achievement."""@en ;
rdfs:comment """In AchievementCredential:The name of the credential for display purposes in wallets. For example, in a list of credentials and in detail views."""@en ;
rdfs:comment """In EndorsementCredential:The name of the credential for display purposes in wallets. For example, in a list of credentials and in detail views."""@en ;
rdfs:comment """In Evidence:A descriptive title of the evidence."""@en ;
rdfs:comment """In Profile:The name of the entity or organization."""@en ;
rdfs:comment """In ResultDescription:The name of the result."""@en ;
rdfs:comment """In RubricCriterionLevel:The name of the rubric criterion level."""@en ;
rdfs:range <https://schema.org/name> ;
rdfs:domain [ owl:unionOf ( <ob:Achievement> <ob:AchievementCredential> <ob:EndorsementCredential> <ob:Evidence> <ob:Profile> <ob:ResultDescription> <ob:RubricCriterionLevel> ) ] ;
rdfs:isDefinedBy <https://purl.imsglobal.org/spec/vc/ob/vocab.html#> ;
.

ob:narrative a rdf:Property ;
rdfs:label "narrative" ;
rdfs:comment """In AchievementSubject:A narrative that connects multiple pieces of evidence. Likely only present at this location if evidence is a multi-value array."""@en ;
rdfs:comment """In Criteria:A narrative of what is needed to earn the achievement. Markdown is allowed."""@en ;
rdfs:comment """In Evidence:A narrative that describes the evidence and process of achievement that led to an assertion."""@en ;
rdfs:domain [ owl:unionOf ( <ob:AchievementSubject> <ob:Criteria> <ob:Evidence> ) ] ;
rdfs:isDefinedBy <https://purl.imsglobal.org/spec/vc/ob/vocab.html#> ;
.

ob:official a rdf:Property ;
rdfs:label "official" ;
rdfs:comment """If the entity is an organization, `official` is the name of an authorized official of the organization."""@en ;
rdfs:domain <ob:Profile> ;
rdfs:isDefinedBy <https://purl.imsglobal.org/spec/vc/ob/vocab.html#> ;
.

ob:otherIdentifier a rdf:Property ;
rdfs:label "otherIdentifier" ;
rdfs:comment """In Achievement:A list of identifiers for the described entity."""@en ;
rdfs:comment """In Profile:A list of identifiers for the described entity."""@en ;
rdfs:range <ob:IdentifierEntry> ;
rdfs:domain [ owl:unionOf ( <ob:Achievement> <ob:Profile> ) ] ;
rdfs:isDefinedBy <https://purl.imsglobal.org/spec/vc/ob/vocab.html#> ;
.

ob:parentOrg a rdf:Property ;
rdfs:label "parentOrg" ;
rdfs:comment """The parent organization of the entity."""@en ;
rdfs:range <ob:Profile> ;
rdfs:domain <ob:Profile> ;
rdfs:isDefinedBy <https://purl.imsglobal.org/spec/vc/ob/vocab.html#> ;
.

ob:patronymicName a rdf:Property ;
rdfs:label "patronymicName" ;
rdfs:comment """Patronymic name."""@en ;
rdfs:domain <ob:Profile> ;
rdfs:isDefinedBy <https://purl.imsglobal.org/spec/vc/ob/vocab.html#> ;
.

ob:phone a rdf:Property ;
rdfs:label "phone" ;
rdfs:comment """A phone number."""@en ;
rdfs:domain <ob:Profile> ;
rdfs:isDefinedBy <https://purl.imsglobal.org/spec/vc/ob/vocab.html#> ;
.

ob:points a rdf:Property ;
rdfs:label "points" ;
rdfs:comment """The points associated with this rubric criterion level."""@en ;
rdfs:domain <ob:RubricCriterionLevel> ;
rdfs:isDefinedBy <https://purl.imsglobal.org/spec/vc/ob/vocab.html#> ;
.

ob:postOfficeBoxNumber a rdf:Property ;
rdfs:label "postOfficeBoxNumber" ;
rdfs:comment """A post office box number for PO box addresses."""@en ;
rdfs:range <https://schema.org/postOfficeBoxNumber> ;
rdfs:domain <ob:Address> ;
rdfs:isDefinedBy <https://purl.imsglobal.org/spec/vc/ob/vocab.html#> ;
.

ob:postalCode a rdf:Property ;
rdfs:label "postalCode" ;
rdfs:comment """A postal code."""@en ;
rdfs:range <https://schema.org/postalCode> ;
rdfs:domain <ob:Address> ;
rdfs:isDefinedBy <https://purl.imsglobal.org/spec/vc/ob/vocab.html#> ;
.

ob:publicKeyMultibase a rdf:Property ;
rdfs:label "publicKeyMultibase" ;
rdfs:comment """The `publicKeyMultibase` property of the verification method MUST be a public key encoded according to [[?MULTICODEC]] and formatted according to [[?MULTIBASE]]. The multicodec encoding of a Ed25519 public key is the two-byte prefix `0xed01` followed by the 32-byte public key data."""@en ;
rdfs:domain <ob:Multikey> ;
rdfs:isDefinedBy <https://purl.imsglobal.org/spec/vc/ob/vocab.html#> ;
.

ob:related a rdf:Property ;
rdfs:label "related" ;
rdfs:comment """The related property identifies another Achievement that should be considered the same for most purposes. It is primarily intended to identify alternate language editions or previous versions of Achievements."""@en ;
rdfs:range <ob:Related> ;
rdfs:domain <ob:Achievement> ;
rdfs:isDefinedBy <https://purl.imsglobal.org/spec/vc/ob/vocab.html#> ;
.

ob:requiredLevel a rdf:Property ;
rdfs:label "requiredLevel" ;
rdfs:comment """The `id` of the rubric criterion level required to pass as determined by the achievement creator."""@en ;
rdfs:domain <ob:ResultDescription> ;
rdfs:isDefinedBy <https://purl.imsglobal.org/spec/vc/ob/vocab.html#> ;
.

ob:requiredValue a rdf:Property ;
rdfs:label "requiredValue" ;
rdfs:comment """A value from `allowedValue` or within the range of `valueMin` to `valueMax` required to pass as determined by the achievement creator."""@en ;
rdfs:domain <ob:ResultDescription> ;
rdfs:isDefinedBy <https://purl.imsglobal.org/spec/vc/ob/vocab.html#> ;
.

ob:result a rdf:Property ;
rdfs:label "result" ;
rdfs:comment """The set of results being asserted."""@en ;
rdfs:range <ob:Result> ;
rdfs:domain <ob:AchievementSubject> ;
rdfs:isDefinedBy <https://purl.imsglobal.org/spec/vc/ob/vocab.html#> ;
.

ob:resultDescription a rdf:Property ;
rdfs:label "resultDescription" ;
rdfs:comment """In Achievement:The set of result descriptions that may be asserted as results with this achievement."""@en ;
rdfs:comment """In Result:An achievement can have many result descriptions describing possible results. The value of `resultDescription` is the `id` of the result description linked to this result. The linked result description must be in the achievement that is being asserted."""@en ;
rdfs:range <ob:ResultDescription> ;
rdfs:domain [ owl:unionOf ( <ob:Achievement> <ob:Result> ) ] ;
rdfs:isDefinedBy <https://purl.imsglobal.org/spec/vc/ob/vocab.html#> ;
.

ob:resultType a rdf:Property ;
rdfs:label "resultType" ;
rdfs:comment """The type of result this description represents. This is an extensible enumerated vocabulary."""@en ;
rdfs:domain <ob:ResultDescription> ;
rdfs:isDefinedBy <https://purl.imsglobal.org/spec/vc/ob/vocab.html#> ;
.

ob:role a rdf:Property ;
rdfs:label "role" ;
rdfs:comment """Role, position, or title of the learner when demonstrating or performing the achievement or evidence of learning being asserted. Examples include 'Student President', 'Intern', 'Captain', etc."""@en ;
rdfs:domain <ob:AchievementSubject> ;
rdfs:isDefinedBy <https://purl.imsglobal.org/spec/vc/ob/vocab.html#> ;
.

ob:rubricCriterionLevel a rdf:Property ;
rdfs:label "rubricCriterionLevel" ;
rdfs:comment """An ordered array of rubric criterion levels that may be asserted in the linked result. The levels should be ordered from low to high as determined by the achievement creator."""@en ;
rdfs:range <ob:RubricCriterionLevel> ;
rdfs:domain <ob:ResultDescription> ;
rdfs:isDefinedBy <https://purl.imsglobal.org/spec/vc/ob/vocab.html#> ;
.

ob:salt a rdf:Property ;
rdfs:label "salt" ;
rdfs:comment """If the `identityHash` is hashed, this should contain the string used to salt the hash. If this value is not provided, it should be assumed that the hash was not salted."""@en ;
rdfs:domain <ob:IdentityObject> ;
rdfs:isDefinedBy <https://purl.imsglobal.org/spec/vc/ob/vocab.html#> ;
.

ob:source a rdf:Property ;
rdfs:label "source" ;
rdfs:comment """The person, organization, or system that assessed the achievement on behalf of the issuer. For example, a school may assess the achievement, while the school district issues the credential."""@en ;
rdfs:range <ob:Profile> ;
rdfs:domain <ob:AchievementSubject> ;
rdfs:isDefinedBy <https://purl.imsglobal.org/spec/vc/ob/vocab.html#> ;
.

ob:specialization a rdf:Property ;
rdfs:label "specialization" ;
rdfs:comment """Name given to the focus, concentration, or specific area of study defined in the achievement. Examples include 'Entrepreneurship', 'Technical Communication', and 'Finance'."""@en ;
rdfs:domain <ob:Achievement> ;
rdfs:isDefinedBy <https://purl.imsglobal.org/spec/vc/ob/vocab.html#> ;
.

ob:status a rdf:Property ;
rdfs:label "status" ;
rdfs:comment """The status of the achievement. Required if `resultType` of the linked ResultDescription is Status."""@en ;
rdfs:domain <ob:Result> ;
rdfs:isDefinedBy <https://purl.imsglobal.org/spec/vc/ob/vocab.html#> ;
.

ob:streetAddress a rdf:Property ;
rdfs:label "streetAddress" ;
rdfs:comment """A street address within the locality."""@en ;
rdfs:range <https://schema.org/streetAddress> ;
rdfs:domain <ob:Address> ;
rdfs:isDefinedBy <https://purl.imsglobal.org/spec/vc/ob/vocab.html#> ;
.

ob:tag a rdf:Property ;
rdfs:label "tag" ;
rdfs:comment """One or more short, human-friendly, searchable, keywords that describe the type of achievement."""@en ;
rdfs:range <https://schema.org/keywords> ;
rdfs:domain <ob:Achievement> ;
rdfs:isDefinedBy <https://purl.imsglobal.org/spec/vc/ob/vocab.html#> ;
.

ob:targetCode a rdf:Property ;
rdfs:label "targetCode" ;
rdfs:comment """If applicable, a locally unique string identifier that identifies the alignment target within its framework and/or targetUrl."""@en ;
rdfs:domain <ob:Alignment> ;
rdfs:isDefinedBy <https://purl.imsglobal.org/spec/vc/ob/vocab.html#> ;
.

ob:targetDescription a rdf:Property ;
rdfs:label "targetDescription" ;
rdfs:comment """Short description of the alignment target."""@en ;
rdfs:range <https://schema.org/targetDescription> ;
rdfs:domain <ob:Alignment> ;
rdfs:isDefinedBy <https://purl.imsglobal.org/spec/vc/ob/vocab.html#> ;
.

ob:targetFramework a rdf:Property ;
rdfs:label "targetFramework" ;
rdfs:comment """Name of the framework the alignment target."""@en ;
rdfs:domain <ob:Alignment> ;
rdfs:isDefinedBy <https://purl.imsglobal.org/spec/vc/ob/vocab.html#> ;
.

ob:targetName a rdf:Property ;
rdfs:label "targetName" ;
rdfs:comment """Name of the alignment."""@en ;
rdfs:range <https://schema.org/targetName> ;
rdfs:domain <ob:Alignment> ;
rdfs:isDefinedBy <https://purl.imsglobal.org/spec/vc/ob/vocab.html#> ;
.

ob:targetType a rdf:Property ;
rdfs:label "targetType" ;
rdfs:comment """The type of the alignment target node."""@en ;
rdfs:domain <ob:Alignment> ;
rdfs:isDefinedBy <https://purl.imsglobal.org/spec/vc/ob/vocab.html#> ;
.

ob:targetUrl a rdf:Property ;
rdfs:label "targetUrl" ;
rdfs:comment """URL linking to the official description of the alignment target, for example an individual standard within an educational framework."""@en ;
rdfs:domain <ob:Alignment> ;
rdfs:isDefinedBy <https://purl.imsglobal.org/spec/vc/ob/vocab.html#> ;
.

ob:term a rdf:Property ;
rdfs:label "term" ;
rdfs:comment """The academic term in which this assertion was achieved."""@en ;
rdfs:domain <ob:AchievementSubject> ;
rdfs:isDefinedBy <https://purl.imsglobal.org/spec/vc/ob/vocab.html#> ;
.

ob:url a rdf:Property ;
rdfs:label "url" ;
rdfs:comment """The homepage or social media profile of the entity, whether individual or institutional. Should be a URL/URI Accessible via HTTP."""@en ;
rdfs:domain <ob:Profile> ;
rdfs:isDefinedBy <https://purl.imsglobal.org/spec/vc/ob/vocab.html#> ;
.

ob:use a rdf:Property ;
rdfs:label "use" ;
rdfs:comment """The `use` (public key use) parameter identifies the intended use of the public key, such as `sig` (signature) or `end` (encryption)."""@en ;
rdfs:domain <ob:JWK> ;
rdfs:isDefinedBy <https://purl.imsglobal.org/spec/vc/ob/vocab.html#> ;
.

ob:value a rdf:Property ;
rdfs:label "value" ;
rdfs:comment """A string representing the result of the performance, or demonstration, of the achievement. For example, 'A' if the recipient received an A grade in class."""@en ;
rdfs:range <https://schema.org/value> ;
rdfs:domain <ob:Result> ;
rdfs:isDefinedBy <https://purl.imsglobal.org/spec/vc/ob/vocab.html#> ;
.

ob:valueMax a rdf:Property ;
rdfs:label "valueMax" ;
rdfs:comment """The maximum possible `value` that may be asserted in a linked result."""@en ;
rdfs:domain <ob:ResultDescription> ;
rdfs:isDefinedBy <https://purl.imsglobal.org/spec/vc/ob/vocab.html#> ;
.

ob:valueMin a rdf:Property ;
rdfs:label "valueMin" ;
rdfs:comment """The minimum possible `value` that may be asserted in a linked result."""@en ;
rdfs:domain <ob:ResultDescription> ;
rdfs:isDefinedBy <https://purl.imsglobal.org/spec/vc/ob/vocab.html#> ;
.

ob:version a rdf:Property ;
rdfs:label "version" ;
rdfs:comment """In Achievement:The version property allows issuers to set a version string for an Achievement. This is particularly useful when replacing a previous version with an update."""@en ;
rdfs:comment """In Related:The version of the related achievement."""@en ;
rdfs:domain [ owl:unionOf ( <ob:Achievement> <ob:Related> ) ] ;
rdfs:isDefinedBy <https://purl.imsglobal.org/spec/vc/ob/vocab.html#> ;
.

ob:x5c a rdf:Property ;
rdfs:label "x5c" ;
rdfs:comment """The `x5c` (X.509 certificate chain) parameter contains a chain of one or more PKIX certificates [[RFC5280]]."""@en ;
rdfs:domain <ob:JWK> ;
rdfs:isDefinedBy <https://purl.imsglobal.org/spec/vc/ob/vocab.html#> ;
.

ob:x5t a rdf:Property ;
rdfs:label "x5t" ;
rdfs:comment """The `x5t` (X.509 certificate SHA-1 thumbprint) parameter is a base64url-encoded SHA-1 thumbprint (a.k.a. digest) of the DER encoding of an X.509 certificate [[RFC5280]]."""@en ;
rdfs:domain <ob:JWK> ;
rdfs:isDefinedBy <https://purl.imsglobal.org/spec/vc/ob/vocab.html#> ;
.

ob:x5t_S256 a rdf:Property ;
rdfs:label "x5t_S256" ;
rdfs:comment """The `x5t#S256` (X.509 certificate SHA-256 thumbprint) parameter is a base64url-encoded SHA-256 thumbprint (a.k.a. digest) of the DER encoding of an X.509 certificate [[RFC5280]]."""@en ;
rdfs:domain <ob:JWK> ;
rdfs:isDefinedBy <https://purl.imsglobal.org/spec/vc/ob/vocab.html#> ;
.

ob:x5u a rdf:Property ;
rdfs:label "x5u" ;
rdfs:comment """The `x5u` (X.509 URL) parameter is a URI that refers to a resource for an X.509 public key certificate or certificate chain [[RFC5280]]."""@en ;
rdfs:domain <ob:JWK> ;
rdfs:isDefinedBy <https://purl.imsglobal.org/spec/vc/ob/vocab.html#> ;
.

